src/State.v
@@ -1,8 +1,8 @@
 
-From mathcomp Require Import ssreflect seq.
+From mathcomp Require Import ssreflect ssrbool eqtype seq.
 From nbits Require Import NBits.
 From ssrlib Require Import Types SsrOrdered Store.
-From BitBlasting Require Import Var.
+From BitBlasting Require Import Var Typ TypEnv.
 
 Set Implicit Arguments.
 Unset Strict Implicit.
@@ -13,4 +13,27 @@ Module ValueType <: HasDefaultTyp.
   Definition default : t := [::].
 End ValueType.
 
-Module State := RealizableTStoreAdapter UVarOrder ValueType.
+Module Store := RealizableTStoreAdapter VarOrder ValueType.
+
+Inductive State : Type :=
+| OK of Store.t
+| ERR.
+
+
+
+(* A store conforms to a typing environment if for every variable, the size of its type
+   in the typing environment is the same as the size of its value in the store *)
+
+Definition conform (s : Store.t) (te : TypEnv.t) : Prop :=
+  forall (v : var) (ty : typ), TypEnv.find v te = Some ty ->
+                               sizeof_typ ty = size (Store.acc v s).
+
+Lemma conform_upd x ty v s te :
+  sizeof_typ ty = size v ->
+  conform s te -> conform (Store.upd x v s) (TypEnv.add x ty te).
+Proof.
+  move=> Hs Hcon y tyy. case Hyx: (y == x).
+  - rewrite (TypEnv.find_add_eq Hyx) (Store.acc_upd_eq Hyx). case=> <-. assumption.
+  - move/idP/negP: Hyx => Hyx. rewrite (TypEnv.find_add_neq Hyx).
+    rewrite (Store.acc_upd_neq Hyx). move=> Hfind. exact: (Hcon y tyy Hfind).
+Qed.
